src/RationalTangles.lean
@@ -16,6 +16,7 @@ import RationalTangles.ColoringInvariance
 import RationalTangles.ColoringR3
 import RationalTangles.ColoringFlype
 import RationalTangles.ColoringIsotopy
+import RationalTangles.ColoringStandard
 import RationalTangles.ColorFraction
 import RationalTangles.Rational
 import RationalTangles.StandardForm
